Mem.v
@@ -1,32 +1,104 @@
+From Coq Require Import Arith.Arith.
+From Coq Require Import Lia.
 From Coq Require Import Lists.List.
 
-Definition mem (A : Type) := list (nat * A). 
+Definition mem (A : Type) := list (nat * A).
 
-Fixpoint get {A : Type} (m : mem A) i default :=
+Fixpoint get {A} default (m : mem A) i :=
   match m with
   | nil => default
-  | (i', a') :: m' => if Nat.eqb i i' then a' else get m' i default 
+  | (i', a') :: m' => if Nat.eqb i i' then a' else get default m' i
   end.
 
-Definition set {A : Type} (m : mem A) i a :=
+Definition set {A} (m : mem A) i a :=
   (i, a) :: m.
 
-Definition length {A : Type} (m : mem A) :=
-  fold_left (fun x y => max x (fst y)) m 0. 
+Local Fixpoint max (n m : nat) :=
+  match n with
+  | 0 => m
+  | S n' => match m with
+            | 0 => n
+            | S m' => S (max n' m')
+            end
+  end.
+
+Fixpoint length {A : Type} (m : mem A) :=
+  match m with
+  | nil => 0
+  | (i, _) :: m' => max i (length m')
+  end.
+
+Definition add {A} (m : mem A) a :=
+  (length m, a) :: m.
 
 (* Proofs *)
 
 Lemma get_set_eq : forall {A} default (m : mem A) i a,
-  get ((i, a) :: m) i default = a.
+  get default ((i, a) :: m) i = a.
 Proof.
   intros. simpl. rewrite PeanoNat.Nat.eqb_refl. reflexivity.
 Qed.
 
-Lemma get_set_neq : forall {A} (m : mem A) i i' a,
+Lemma get_set_neq : forall {A} default (m : mem A) i i' a,
   i <> i' ->
-  get ((i', a) :: m) i = get m i.
+  get default ((i', a) :: m) i = get default m i.
 Proof.
   intros * Hneq. eapply PeanoNat.Nat.eqb_neq in Hneq.
   simpl. rewrite Hneq. reflexivity.
+Qed.
+
+Lemma get_add_eq : forall {A} default (m : mem A) a,
+  get default (add m a) (length m) = a.
+Proof.
+  intros. unfold add. eauto using get_set_eq.
+Qed.
+
+Lemma get_add_lt : forall {A} default (m : mem A) a i,
+  i < length m ->
+  get default (add m a) i = get default m i.
+Proof.
+  intros. simpl. destruct (Nat.eqb _ _) eqn:E; trivial. 
+  eapply Nat.eqb_eq in E. lia.
+Qed.
+
+Lemma get_add_gt : forall {A} default (m : mem A) a i,
+  length m < i ->
+  get default (add m a) i = default.
+Proof.
+  intros * H. simpl. destruct (Nat.eqb _ _) eqn:E.
+  - eapply Nat.eqb_eq in E. lia.
+  - clear E. unfold length in *.
+    induction m as [| [i' a'] m]; trivial.
+    fold (@length A) in *.
+    destruct (Nat.eq_dec i i'); subst.
+    + rewrite get_set_eq.
+
+    induction m as [| [i' a'] m]; trivial.
+    simpl. destruct (i =? i') eqn:E.
+    + eapply Nat.eqb_eq in E; subst.
+Admitted.
+
+Lemma set_preserves_memory_length : forall {A} (m : mem A) i a,
+  i < length m ->
+  length m = length (set m i a).
+Proof.
+  intros * H. unfold set.
+  destruct m as [|[i' a'] m]; try solve [inversion H].
+  assert (forall x y, x < y -> y = max x y). {
+    intros x. induction x; eauto.
+    intros y. destruct y; try lia.
+    eauto using eq_S, Lt.lt_S_n.
+  }
+  eauto.
+Qed.
+
+Lemma add_increments_memory_length : forall {A} (m : mem A) a,
+  length (add m a) = length m.
+Proof.
+  intros. destruct m as [|[i a'] m]; trivial.
+  simpl. destruct (max i (length m)); trivial.
+  assert (forall x, max (S x) (S x) = S x).
+  { intros. unfold max. induction x; eauto. }
+  eauto.
 Qed.
 
